Foundation/Modal/Hilbert2/MaximalConsistentSet.lean
@@ -1,4 +1,4 @@
-import Foundation.Modal.Hilbert.Basic
+import Foundation.Modal.Hilbert2.Basic
 
 namespace LO.Modal
 
@@ -8,15 +8,11 @@ variable {H : Hilbert α}
 open System
 open Hilbert.Deduction
 
-abbrev FormulaSet.Consistent (H : Hilbert α) (T : FormulaSet α) := T *⊬[H] ⊥
-
-abbrev FormulaSet.Inconsistent (H : Hilbert α) (T : FormulaSet α) := ¬(T.Consistent H)
-
 namespace FormulaSet
 
-variable {T : FormulaSet α} (T_consis : T.Consistent H)
+variable {T : FormulaSet α} (T_consis : T *⊬[H] ⊥)
 
-lemma def_consistent : T.Consistent H ↔ ∀ (Γ : List (Formula α)), (∀ ψ ∈ Γ, ψ ∈ T) → Γ ⊬[H] ⊥ := by
+lemma def_consistent : T *⊬[H] ⊥ ↔ ∀ (Γ : List (Formula α)), (∀ ψ ∈ Γ, ψ ∈ T) → Γ ⊬[H] ⊥ := by
   constructor;
   . intro h;
     simpa using Context.provable_iff.not.mp h;
@@ -24,9 +20,12 @@ lemma def_consistent : T.Consistent H ↔ ∀ (Γ : List (Formula α)), (∀ ψ 
     apply Context.provable_iff.not.mpr; push_neg;
     assumption;
 
-lemma def_inconsistent : ¬T.Consistent H ↔ ∃ (Γ : List (Formula α)), (∀ ψ ∈ Γ, ψ ∈ T) ∧ Γ ⊢[H]! ⊥ := by
-  simp only [def_consistent]; push_neg; tauto;
+lemma def_inconsistent : T *⊢[H]! ⊥ ↔ ∃ (Γ : List (Formula α)), (∀ ψ ∈ Γ, ψ ∈ T) ∧ Γ ⊢[H]! ⊥ := by
+  apply not_iff_not.mp;
+  push_neg;
+  exact def_consistent;
 
+/-
 @[simp]
 lemma self_consistent [H_consis : System.Consistent H] : H.axioms.Consistent H := by
   obtain ⟨ψ, hq⟩ := H_consis.exists_unprovable;
@@ -35,17 +34,18 @@ lemma self_consistent [H_consis : System.Consistent H] : H.axioms.Consistent H :
   by_contra hC;
   have : H ⊢! ψ := imp_trans''! hC efq! ⨀ (iff_provable_list_conj.mpr $ λ _ h => maxm! $ hΓ _ h);
   contradiction;
+-/
 
-lemma union_consistent : FormulaSet.Consistent H (T₁ ∪ T₂) → T₁.Consistent H ∧ T₂.Consistent H := by
+lemma union_consistent : (T₁ ∪ T₂) *⊬[H] ⊥ → T₁ *⊬[H] ⊥ ∧ T₂ *⊬[H] ⊥ := by
   intro h;
   replace h := def_consistent.mp h;
-  constructor <;> { apply def_consistent.mpr; intro Γ hΓ; exact h Γ (by simp_all); }
+  constructor <;> {
+    apply def_consistent.mpr;
+    intro Γ hΓ;
+    exact h Γ $ by tauto_set;
+  }
 
-lemma union_not_consistent : ¬T₁.Consistent H ∨ ¬T₂.Consistent H → ¬(FormulaSet.Consistent H (T₁ ∪ T₂)) := by
-  contrapose; push_neg;
-  exact union_consistent;
-
-lemma emptyset_consistent [H_consis : System.Consistent H] : FormulaSet.Consistent H ∅ := by
+lemma emptyset_consistent [H_consis : System.Consistent H] : ∅ *⊬[H] ⊥ := by
   obtain ⟨f, hf⟩ := H_consis.exists_unprovable;
   apply def_consistent.mpr;
   intro Γ hΓ; by_contra hC;
@@ -55,7 +55,7 @@ lemma emptyset_consistent [H_consis : System.Consistent H] : FormulaSet.Consiste
 
 variable [DecidableEq α]
 
-lemma iff_insert_consistent : FormulaSet.Consistent H (insert φ T) ↔ ∀ {Γ : List (Formula α)}, (∀ ψ ∈ Γ, ψ ∈ T) → H ⊬ φ ⋏ ⋀Γ ➝ ⊥ := by
+lemma iff_insert_consistent : (insert φ T) *⊬[H] ⊥ ↔ ∀ {Γ : List (Formula α)}, (∀ ψ ∈ Γ, ψ ∈ T) → H ⊬ φ ⋏ ⋀Γ ➝ ⊥ := by
   constructor;
   . intro h Γ hΓ;
     by_contra hC;
@@ -82,12 +82,12 @@ lemma iff_insert_consistent : FormulaSet.Consistent H (insert φ T) ↔ ∀ {Γ 
     have := imp_trans''! and_comm! $ imply_left_remove_conj! (φ := φ) $ FiniteContext.provable_iff.mp hC;
     contradiction;
 
-lemma iff_insert_inconsistent : ¬(insert φ T).Consistent H ↔ ∃ Γ : List (Formula α), (∀ φ ∈ Γ, φ ∈ T) ∧ H ⊢! φ ⋏ ⋀Γ ➝ ⊥ := by
-  constructor;
-  . contrapose; push_neg; apply iff_insert_consistent.mpr;
-  . contrapose; push_neg; apply iff_insert_consistent.mp;
+lemma iff_insert_inconsistent : (insert φ T) *⊢[H]! ⊥ ↔ ∃ Γ : List (Formula α), (∀ φ ∈ Γ, φ ∈ T) ∧ H ⊢! φ ⋏ ⋀Γ ➝ ⊥ := by
+  apply not_iff_not.mp;
+  push_neg;
+  exact iff_insert_consistent;
 
-lemma provable_iff_insert_neg_not_consistent : T *⊢[H]! φ ↔ ¬FormulaSet.Consistent H (insert (∼φ) T) := by
+lemma provable_iff_insert_neg_not_consistent : T *⊢[H]! φ ↔ (insert (∼φ) T) *⊢[H]! ⊥ := by
   constructor;
   . intro h;
     apply iff_insert_inconsistent.mpr;
@@ -107,16 +107,16 @@ lemma provable_iff_insert_neg_not_consistent : T *⊢[H]! φ ↔ ¬FormulaSet.Co
     . have : Γ ⊢[H]! ∼φ ➝ ⊥ := imp_swap'! $ and_imply_iff_imply_imply'!.mp hΓ₂;
       exact dne'! $ neg_equiv'!.mpr this;
 
-lemma unprovable_iff_insert_neg_consistent : T *⊬[H] φ ↔ FormulaSet.Consistent H (insert (∼φ) T) := by
+lemma unprovable_iff_insert_neg_consistent : T *⊬[H] φ ↔ (insert (∼φ) T) *⊬[H] ⊥ := by
   simpa [not_not] using provable_iff_insert_neg_not_consistent.not;
 
-lemma unprovable_iff_singleton_neg_consistent : H ⊬ φ ↔ FormulaSet.Consistent H {∼φ} := by
+lemma unprovable_iff_singleton_neg_consistent : H ⊬ φ ↔ {∼φ} *⊬[H] ⊥ := by
   have e : insert (∼φ) ∅ = ({∼φ} : FormulaSet α) := by aesop;
-  have H := unprovable_iff_insert_neg_consistent (H := H) (T := ∅) (φ := φ);
-  rw [e] at H;
-  exact Iff.trans Context.provable_iff_provable.not H;
+  have h₂ := unprovable_iff_insert_neg_consistent (H := H) (T := ∅) (φ := φ);
+  rw [e] at h₂;
+  exact Iff.trans Context.provable_iff_provable.not h₂;
 
-lemma neg_provable_iff_insert_not_consistent : T *⊢[H]! ∼φ ↔ ¬FormulaSet.Consistent H (insert (φ) T) := by
+lemma neg_provable_iff_insert_not_consistent : T *⊢[H]! ∼φ ↔ (insert (φ) T) *⊢[H]! ⊥ := by
   constructor;
   . intro h;
     apply iff_insert_inconsistent.mpr;
@@ -136,36 +136,37 @@ lemma neg_provable_iff_insert_not_consistent : T *⊢[H]! ∼φ ↔ ¬FormulaSet
     . apply neg_equiv'!.mpr;
       exact imp_swap'! $ and_imply_iff_imply_imply'!.mp hΓ₂;
 
-lemma neg_unprovable_iff_insert_consistent : T *⊬[H] ∼φ ↔ FormulaSet.Consistent H (insert (φ) T) := by
+lemma neg_unprovable_iff_insert_consistent : T *⊬[H] ∼φ ↔ (insert (φ) T) *⊬[H] ⊥ := by
   simpa [not_not] using neg_provable_iff_insert_not_consistent.not;
 
-lemma unprovable_iff_singleton_consistent : H ⊬ ∼φ ↔ FormulaSet.Consistent H {φ} := by
+lemma unprovable_iff_singleton_consistent : H ⊬ ∼φ ↔ {φ} *⊬[H] ⊥ := by
   have e : insert (φ) ∅ = ({φ} : FormulaSet α) := by aesop;
-  have H := neg_unprovable_iff_insert_consistent (H := H) (T := ∅) (φ := φ);
-  rw [e] at H;
-  exact Iff.trans Context.provable_iff_provable.not H;
+  have h₂ := neg_unprovable_iff_insert_consistent (H := H) (T := ∅) (φ := φ);
+  rw [e] at h₂;
+  exact Iff.trans Context.provable_iff_provable.not h₂;
 
+/-
 omit [DecidableEq α] in
 lemma unprovable_falsum (T_consis : T.Consistent H) : T *⊬[H] ⊥ := by
   by_contra hC;
   obtain ⟨Γ, hΓ₁, _⟩ := Context.provable_iff.mp $ hC;
   have : Γ ⊬[H] ⊥ := (def_consistent.mp T_consis) _ hΓ₁;
   contradiction;
+-/
 
-lemma unprovable_either (T_consis : T.Consistent H) : ¬(T *⊢[H]! φ ∧ T *⊢[H]! ∼φ) := by
+lemma unprovable_either (T_consis : T *⊬[H] ⊥) : ¬(T *⊢[H]! φ ∧ T *⊢[H]! ∼φ) := by
   by_contra hC;
   have ⟨hC₁, hC₂⟩ := hC;
   have : T *⊢[H]! ⊥ := neg_mdp! hC₂ hC₁;
-  have : T *⊬[H] ⊥ := unprovable_falsum T_consis;
   contradiction;
 
-lemma not_mem_falsum_of_consistent (T_consis : T.Consistent H) : ⊥ ∉ T := by
+lemma not_mem_falsum_of_consistent (T_consis : T *⊬[H] ⊥) : ⊥ ∉ T := by
   by_contra hC;
   have : H ⊬ ⊥ ➝ ⊥ := (def_consistent.mp T_consis) [⊥] (by simpa);
   have : H ⊢! ⊥ ➝ ⊥ := efq!;
   contradiction;
 
-lemma not_singleton_consistent [H.HasNecessitation] (T_consis : T.Consistent H) (h : ∼□φ ∈ T) : FormulaSet.Consistent H {∼φ} := by
+lemma not_singleton_consistent (T_consis : T *⊬[H] ⊥) (h : ∼□φ ∈ T) : {∼φ} *⊬[H] ⊥ := by
   apply def_consistent.mpr;
   intro Γ hΓ;
   simp only [Set.mem_singleton_iff] at hΓ;
@@ -174,25 +175,25 @@ lemma not_singleton_consistent [H.HasNecessitation] (T_consis : T.Consistent H) 
   have : H ⊬ ∼(□φ) ➝ ⊥ := def_consistent.mp T_consis (Γ := [∼(□φ)]) (by aesop)
   contradiction;
 
-lemma either_consistent (T_consis : T.Consistent H) (φ) : FormulaSet.Consistent H (insert φ T) ∨ FormulaSet.Consistent H (insert (∼φ) T) := by
-  by_contra hC; push_neg at hC;
-  obtain ⟨Γ, hΓ₁, hΓ₂⟩ := iff_insert_inconsistent.mp hC.1;
-  obtain ⟨Δ, hΔ₁, hΔ₂⟩ := iff_insert_inconsistent.mp hC.2;
-
+lemma either_consistent (T_consis : T *⊬[H] ⊥) (φ) : (insert φ T) *⊬[H] ⊥ ∨ (insert (∼φ) T) *⊬[H] ⊥ := by
+  by_contra hC;
+  push_neg at hC;
+  obtain ⟨hC₁, hC₂⟩ := hC
+  obtain ⟨Γ, hΓ₁, hΓ₂⟩ := iff_insert_inconsistent.mp $ by simpa using hC₁;
+  obtain ⟨Δ, hΔ₁, hΔ₂⟩ := iff_insert_inconsistent.mp $ by simpa using hC₂;
   replace hΓ₂ := neg_equiv'!.mpr hΓ₂;
   replace hΔ₂ := neg_equiv'!.mpr hΔ₂;
   have : H ⊢! ⋀Γ ⋏ ⋀Δ ➝ ⊥ := neg_equiv'!.mp $ demorgan₁'! $ or₃'''! (imp_trans''! (imply_of_not_or'! $ demorgan₄'! hΓ₂) or₁!) (imp_trans''! (imply_of_not_or'! $ demorgan₄'! hΔ₂) or₂!) lem!
   have : H ⊬ ⋀Γ ⋏ ⋀Δ ➝ ⊥ := unprovable_imp_trans''! imply_left_concat_conj! $ def_consistent.mp T_consis (Γ ++ Δ) $ by
-    simp;
+    simp only [List.mem_append];
     rintro ψ (hqΓ | hqΔ);
     . exact hΓ₁ ψ hqΓ;
     . exact hΔ₁ ψ hqΔ;
   contradiction;
 
-lemma exists_maximal_consistent_theory
-  (T_consis : T.Consistent H)
-  : ∃ Z, FormulaSet.Consistent H Z ∧ T ⊆ Z ∧ ∀ U, FormulaSet.Consistent H U → Z ⊆ U → U = Z := by
-  obtain ⟨Z, h₁, ⟨h₂, h₃⟩⟩ := zorn_subset_nonempty { T : FormulaSet α | T.Consistent H } (by
+lemma exists_consistent_maximal_of_consistent (T_consis : T *⊬[H] ⊥)
+  : ∃ Z, Z *⊬[H] ⊥ ∧ T ⊆ Z ∧ ∀ U, U *⊬[H] ⊥ → Z ⊆ U → U = Z := by
+  obtain ⟨Z, h₁, ⟨h₂, h₃⟩⟩ := zorn_subset_nonempty { T : FormulaSet α | T *⊬[H] ⊥ } (by
     intro c hc chain hnc;
     existsi (⋃₀ c);
     simp only [Set.mem_setOf_eq, Set.mem_sUnion];
@@ -204,8 +205,8 @@ lemma exists_maximal_consistent_theory
           (s := ↑Γ.toFinset) (by simp)
           (by intro φ hp; simp_all);
       simp [List.coe_toFinset] at hUs;
-      have : FormulaSet.Consistent H U := hc hUc;
-      have : ¬FormulaSet.Consistent H U := by
+      have : U *⊬[H] ⊥ := hc hUc;
+      have : U *⊢[H]! ⊥ := by
         apply def_inconsistent.mpr;
         use Γ;
         constructor;
@@ -223,12 +224,12 @@ lemma exists_maximal_consistent_theory
     apply Set.eq_of_subset_of_subset;
     . exact h₃ hU hZU;
     . assumption;
-protected alias lindenbaum := exists_maximal_consistent_theory
+protected alias lindenbaum := exists_consistent_maximal_of_consistent
 
 omit [DecidableEq α] in
 open Classical in
 lemma intro_union_consistent
-  (h : ∀ {Γ₁ Γ₂ : List (Formula α)}, (∀ φ ∈ Γ₁, φ ∈ T₁) ∧ (∀ φ ∈ Γ₂, φ ∈ T₂) → H ⊬ ⋀Γ₁ ⋏ ⋀Γ₂ ➝ ⊥) : FormulaSet.Consistent H (T₁ ∪ T₂) := by
+  (h : ∀ {Γ₁ Γ₂ : List (Formula α)}, (∀ φ ∈ Γ₁, φ ∈ T₁) ∧ (∀ φ ∈ Γ₂, φ ∈ T₂) → H ⊬ ⋀Γ₁ ⋏ ⋀Γ₂ ➝ ⊥) : (T₁ ∪ T₂) *⊬[H] ⊥ := by
   apply def_consistent.mpr;
   intro Δ hΔ;
   let Δ₁ := (Δ.filter (· ∈ T₁));
@@ -246,7 +247,7 @@ lemma intro_union_consistent
 open Classical in
 lemma intro_triunion_consistent
   (h : ∀ {Γ₁ Γ₂ Γ₃ : List (Formula α)}, (∀ φ ∈ Γ₁, φ ∈ T₁) ∧ (∀ φ ∈ Γ₂, φ ∈ T₂) ∧ (∀ φ ∈ Γ₃, φ ∈ T₃) → H ⊬ ⋀Γ₁ ⋏ ⋀Γ₂ ⋏ ⋀Γ₃ ➝ ⊥)
-  : FormulaSet.Consistent H (T₁ ∪ T₂ ∪ T₃) := by
+  : (T₁ ∪ T₂ ∪ T₃) *⊬[H] ⊥ := by
   apply intro_union_consistent;
   rintro Γ₁₂ Γ₃ ⟨h₁₂, h₃⟩;
   simp at h₁₂;
@@ -257,7 +258,8 @@ lemma intro_triunion_consistent
       apply and_replace_left!;
       apply imply_left_conj_concat!.mp;
       apply conjconj_subset!;
-      intro φ hp; simp [Γ₁, Γ₂];
+      intro φ hp;
+      simp [Γ₁, Γ₂];
       rcases h₁₂ φ hp with (h₁ | h₂);
       . left; exact ⟨hp, h₁⟩;
       . right; exact ⟨hp, h₂⟩;
@@ -273,109 +275,107 @@ lemma intro_triunion_consistent
         simpa using List.of_mem_filter hp;
       . assumption;
 
-lemma not_mem_of_mem_neg (T_consis : T.Consistent H) (h : ∼φ ∈ T) : φ ∉ T := by
+lemma not_mem_of_mem_neg (T_consis : T *⊬[H] ⊥) (h : ∼φ ∈ T) : φ ∉ T := by
   by_contra hC;
   have : [φ, ∼φ] ⊬[H] ⊥ := (FormulaSet.def_consistent.mp T_consis) [φ, ∼φ] (by simp_all);
   have : [φ, ∼φ] ⊢[H]! ⊥ := System.bot_of_mem_either! (φ := φ) (Γ := [φ, ∼φ]) (by simp) (by simp);
   contradiction;
 
-lemma not_mem_neg_of_mem (T_consis : T.Consistent H) (h : φ ∈ T) : ∼φ ∉ T := by
+lemma not_mem_neg_of_mem (T_consis : T *⊬[H] ⊥) (h : φ ∈ T) : ∼φ ∉ T := by
   by_contra hC;
   have : [φ, ∼φ] ⊬[H] ⊥ := (FormulaSet.def_consistent.mp T_consis) [φ, ∼φ] (by simp_all);
   have : [φ, ∼φ] ⊢[H]! ⊥ := System.bot_of_mem_either! (φ := φ) (Γ := [φ, ∼φ]) (by simp) (by simp);
   contradiction;
 end FormulaSet
 
-structure MaximalConsistentFormulaSet (H : Hilbert α) where
-  theory : FormulaSet α
-  consistent : theory.Consistent H
-  maximal : ∀ {U}, theory ⊂ U → ¬FormulaSet.Consistent H U
-alias MCT := MaximalConsistentFormulaSet
+abbrev MaximalConsistentSet (H : Hilbert α) := { T : FormulaSet α // (T *⊬[H] ⊥) ∧ (∀ {U}, T ⊂ U → U *⊢[H]! ⊥)}
 
-namespace MaximalConsistentFormulaSet
+alias MCS := MaximalConsistentSet
+
+namespace MaximalConsistentSet
 
 open FormulaSet
 
+lemma consistent {Ω : MCS H} : Ω.1 *⊬[H] ⊥ := Ω.2.1
+
+lemma maximal {Ω : MCS H} : Ω.1 ⊂ U → U *⊢[H]! ⊥ := Ω.2.2
+
 variable [DecidableEq α]
 variable {H : Hilbert α}
-variable {Ω Ω₁ Ω₂ : MCT H}
+variable {Ω Ω₁ Ω₂ : MCS H}
 variable {φ : Formula α}
 
-lemma exists_maximal_Lconsistented_theory (consisT : T.Consistent H) : ∃ Ω : MCT H, (T ⊆ Ω.theory) := by
+instance : Membership (Formula α) (MCS H) := ⟨λ Ω φ => φ ∈ Ω.1⟩
+
+lemma exists_of_consistent {T : FormulaSet α} (consisT : T *⊬[H] ⊥) : ∃ Ω : MCS H, (T ⊆ Ω.1) := by
   have ⟨Ω, hΩ₁, hΩ₂, hΩ₃⟩ := FormulaSet.lindenbaum consisT;
-  use {
-    theory := Ω,
-    consistent := hΩ₁,
-    maximal := by
-      rintro U ⟨hU₁, hU₂⟩;
-      by_contra hC;
-      have : U = Ω := hΩ₃ U hC hU₁;
-      subst_vars;
-      simp at hU₂,
-  }
+  use ⟨Ω, ?_, ?_⟩;
+  . assumption;
+  . rintro U ⟨hU₁, _⟩;
+    by_contra hC;
+    have := hΩ₃ U hC $ hU₁;
+    subst this;
+    simp_all;
 
-alias lindenbaum := exists_maximal_Lconsistented_theory
+alias lindenbaum := exists_of_consistent
 
-instance [System.Consistent H] : Nonempty (MCT H) := ⟨lindenbaum emptyset_consistent |>.choose⟩
+instance [System.Consistent H] : Nonempty (MCS H) := ⟨lindenbaum emptyset_consistent |>.choose⟩
 
-lemma either_mem (Ω : MCT H) (φ) : φ ∈ Ω.theory ∨ ∼φ ∈ Ω.theory := by
+lemma either_mem (Ω : MCS H) (φ) : φ ∈ Ω ∨ ∼φ ∈ Ω := by
   by_contra hC; push_neg at hC;
-  cases either_consistent Ω.consistent φ with
-  | inl h => have := Ω.maximal (Set.ssubset_insert hC.1); contradiction;
-  | inr h => have := Ω.maximal (Set.ssubset_insert hC.2); contradiction;
+  cases either_consistent consistent φ with
+  | inl h => have := maximal (Set.ssubset_insert hC.1); contradiction;
+  | inr h => have := maximal (Set.ssubset_insert hC.2); contradiction;
 
 omit [DecidableEq α] in
-lemma maximal' {φ : Formula α} (hp : φ ∉ Ω.theory) : ¬FormulaSet.Consistent H (insert φ Ω.theory) := Ω.maximal (Set.ssubset_insert hp)
+lemma maximal' {φ : Formula α} (hp : φ ∉ Ω) : (insert φ Ω.1) *⊢[H]! ⊥ := maximal (Set.ssubset_insert hp)
 
-lemma membership_iff : (φ ∈ Ω.theory) ↔ (Ω.theory *⊢[H]! φ) := by
+lemma membership_iff : (φ ∈ Ω) ↔ (Ω.1 *⊢[H]! φ) := by
   constructor;
   . intro h; exact Context.by_axm! h;
   . intro hp;
-    suffices ∼φ ∉ Ω.theory by apply or_iff_not_imp_right.mp $ (either_mem Ω φ); assumption;
+    suffices ∼φ ∉ Ω.1 by apply or_iff_not_imp_right.mp $ (either_mem Ω φ); assumption;
     by_contra hC;
-    have hnp : Ω.theory *⊢[H]! ∼φ := Context.by_axm! hC;
-    have := neg_mdp! hnp hp;
-    have := Ω.consistent;
+    have hnp : Ω.1 *⊢[H]! ∼φ := Context.by_axm! hC;
+    have : Ω.1 *⊢[H]! ⊥ := neg_mdp! hnp hp;
+    have : Ω.1 *⊬[H] ⊥ := consistent;
     contradiction;
 
-lemma subset_axiomset : H.axioms ⊆ Ω.theory := by
+lemma subset_axiomset : H.axioms ⊆ Ω.1 := by
   intro φ hp;
   apply membership_iff.mpr;
   apply Context.of!;
   exact maxm! (by aesop);
 
-@[simp] lemma not_mem_falsum : ⊥ ∉ Ω.theory := not_mem_falsum_of_consistent Ω.consistent
+@[simp] lemma not_mem_falsum : ⊥ ∉ Ω.1 := not_mem_falsum_of_consistent consistent
 
-@[simp] lemma mem_verum : ⊤ ∈ Ω.theory := by apply membership_iff.mpr; apply verum!;
-
-@[simp]
-lemma unprovable_falsum : Ω.theory *⊬[H] ⊥ := by apply membership_iff.not.mp; simp
+@[simp] lemma mem_verum : ⊤ ∈ Ω := by apply membership_iff.mpr; apply verum!;
 
 @[simp]
-lemma iff_mem_neg : (∼φ ∈ Ω.theory) ↔ (φ ∉ Ω.theory) := by
+lemma iff_mem_neg : (∼φ ∈ Ω) ↔ (φ ∉ Ω.1) := by
   constructor;
   . intro hnp;
     by_contra hp;
     replace hp := membership_iff.mp hp;
     replace hnp := membership_iff.mp hnp;
-    have : Ω.theory *⊢[H]! ⊥ := neg_mdp! hnp hp;
-    have : Ω.theory *⊬[H] ⊥ := unprovable_falsum;
+    have : Ω.1 *⊢[H]! ⊥ := neg_mdp! hnp hp;
+    have : Ω.1 *⊬[H] ⊥ := consistent;
     contradiction;
   . intro hp;
     have := provable_iff_insert_neg_not_consistent.not.mp $ membership_iff.not.mp hp;
-    have := (not_imp_not.mpr $ Ω.maximal (U := insert (∼φ) Ω.theory)) this;
-    have : insert (∼φ) Ω.theory ⊆ Ω.theory := by simpa [Set.ssubset_def] using this;
+    have := not_imp_not.mpr (@maximal (Ω := Ω) (U := insert (∼φ) Ω.1)) this;
+    have : insert (∼φ) Ω.1 ⊆ Ω.1 := by simpa [Set.ssubset_def] using this;
     apply this;
     tauto_set;
 
-lemma iff_mem_negneg : (∼∼φ ∈ Ω.theory) ↔ (φ ∈ Ω.theory) := by
+lemma iff_mem_negneg : (∼∼φ ∈ Ω) ↔ (φ ∈ Ω) := by
   simp only [membership_iff];
   constructor;
-  . exact dne'!;
-  . exact dni'!;
+  . apply dne'!;
+  . apply dni'!;
 
 @[simp]
-lemma iff_mem_imp : ((φ ➝ ψ) ∈ Ω.theory) ↔ (φ ∈ Ω.theory) → (ψ ∈ Ω.theory) := by
+lemma iff_mem_imp : ((φ ➝ ψ) ∈ Ω) ↔ (φ ∈ Ω) → (ψ ∈ Ω) := by
   constructor;
   . intro hpq hp;
     replace dpq := membership_iff.mp hpq;
@@ -383,7 +383,7 @@ lemma iff_mem_imp : ((φ ➝ ψ) ∈ Ω.theory) ↔ (φ ∈ Ω.theory) → (ψ �
     apply membership_iff.mpr;
     exact dpq ⨀ dp;
   . intro h;
-    replace h : φ ∉ Ω.theory ∨ ψ ∈ Ω.theory := or_iff_not_imp_left.mpr (by simpa using h);
+    replace h : φ ∉ Ω.1 ∨ ψ ∈ Ω := or_iff_not_imp_left.mpr (by simpa using h);
     cases h with
     | inl h =>
       apply membership_iff.mpr;
@@ -393,7 +393,7 @@ lemma iff_mem_imp : ((φ ➝ ψ) ∈ Ω.theory) ↔ (φ ∈ Ω.theory) → (ψ �
       exact imply₁! ⨀ (membership_iff.mp h)
 
 @[simp]
-lemma iff_mem_and : ((φ ⋏ ψ) ∈ Ω.theory) ↔ (φ ∈ Ω.theory) ∧ (ψ ∈ Ω.theory) := by
+lemma iff_mem_and : ((φ ⋏ ψ) ∈ Ω) ↔ (φ ∈ Ω) ∧ (ψ ∈ Ω) := by
   constructor;
   . intro hpq;
     replace hpq := membership_iff.mp hpq;
@@ -405,7 +405,7 @@ lemma iff_mem_and : ((φ ⋏ ψ) ∈ Ω.theory) ↔ (φ ∈ Ω.theory) ∧ (ψ �
     exact and₃'! (membership_iff.mp hp) (membership_iff.mp hq);
 
 @[simp]
-lemma iff_mem_or : ((φ ⋎ ψ) ∈ Ω.theory) ↔ (φ ∈ Ω.theory) ∨ (ψ ∈ Ω.theory) := by
+lemma iff_mem_or : ((φ ⋎ ψ) ∈ Ω) ↔ (φ ∈ Ω) ∨ (ψ ∈ Ω) := by
   constructor;
   . intro hpq;
     replace hpq := membership_iff.mp hpq;
@@ -414,8 +414,8 @@ lemma iff_mem_or : ((φ ⋎ ψ) ∈ Ω.theory) ↔ (φ ∈ Ω.theory) ∨ (ψ �
     have ⟨hp, hq⟩ := hC;
     replace hp := membership_iff.mp $ iff_mem_neg.mpr hp;
     replace hq := membership_iff.mp $ iff_mem_neg.mpr hq;
-    have : Ω.theory *⊢[H]! ⊥ := or₃'''! (neg_equiv'!.mp hp) (neg_equiv'!.mp hq) hpq;
-    have : Ω.theory *⊬[H] ⊥ := unprovable_falsum;
+    have : Ω.1 *⊢[H]! ⊥ := or₃'''! (neg_equiv'!.mp hp) (neg_equiv'!.mp hq) hpq;
+    have : Ω.1 *⊬[H] ⊥ := consistent;
     contradiction;
   . rintro (hp | hq);
     . apply membership_iff.mpr;
@@ -423,21 +423,21 @@ lemma iff_mem_or : ((φ ⋎ ψ) ∈ Ω.theory) ↔ (φ ∈ Ω.theory) ∨ (ψ �
     . apply membership_iff.mpr;
       exact or₂'! (membership_iff.mp hq);
 
-lemma iff_congr : (Ω.theory *⊢[H]! (φ ⭤ ψ)) → ((φ ∈ Ω.theory) ↔ (ψ ∈ Ω.theory)) := by
+lemma iff_congr : (Ω.1 *⊢[H]! (φ ⭤ ψ)) → ((φ ∈ Ω) ↔ (ψ ∈ Ω)) := by
   intro hpq;
   constructor;
   . intro hp; exact iff_mem_imp.mp (membership_iff.mpr $ and₁'! hpq) hp;
   . intro hq; exact iff_mem_imp.mp (membership_iff.mpr $ and₂'! hpq) hq;
 
-lemma mem_dn_iff : (φ ∈ Ω.theory) ↔ (∼∼φ ∈ Ω.theory) := iff_congr $ dn!
+lemma mem_dn_iff : (φ ∈ Ω) ↔ (∼∼φ ∈ Ω) := iff_congr $ dn!
 
 omit [DecidableEq α] in
-lemma equality_def : Ω₁ = Ω₂ ↔ Ω₁.theory = Ω₂.theory := by
+lemma equality_def : Ω₁ = Ω₂ ↔ Ω₁.1 = Ω₂.1 := by
   constructor;
   . intro h; cases h; rfl;
   . intro h; cases Ω₁; cases Ω₂; simp_all;
 
-lemma intro_equality {h : ∀ φ, φ ∈ Ω₁.theory → φ ∈ Ω₂.theory} : Ω₁ = Ω₂ := by
+lemma intro_equality {h : ∀ φ, φ ∈ Ω₁.1 → φ ∈ Ω₂.1} : Ω₁ = Ω₂ := by
   exact equality_def.mpr $ Set.eq_of_subset_of_subset
     (by intro φ hp; exact h φ hp)
     (by
@@ -449,7 +449,7 @@ lemma intro_equality {h : ∀ φ, φ ∈ Ω₁.theory → φ ∈ Ω₂.theory} :
       apply iff_mem_neg.mpr hp;
     )
 
-lemma neg_imp (h : ψ ∈ Ω₂.theory → φ ∈ Ω₁.theory) : (∼φ ∈ Ω₁.theory) → (∼ψ ∈ Ω₂.theory) := by
+lemma neg_imp (h : ψ ∈ Ω₂.1 → φ ∈ Ω₁.1) : (∼φ ∈ Ω₁.1) → (∼ψ ∈ Ω₂.1) := by
   contrapose;
   intro hq;
   apply iff_mem_neg.mp;
@@ -457,20 +457,22 @@ lemma neg_imp (h : ψ ∈ Ω₂.theory → φ ∈ Ω₁.theory) : (∼φ ∈ Ω�
   apply h;
   exact mem_dn_iff.mpr $ iff_mem_neg.mpr hq;
 
-lemma neg_iff (h : φ ∈ Ω₁.theory ↔ ψ ∈ Ω₂.theory) : (∼φ ∈ Ω₁.theory) ↔ (∼ψ ∈ Ω₂.theory) := ⟨neg_imp $ h.mpr, neg_imp $ h.mp⟩
+lemma neg_iff (h : φ ∈ Ω₁.1 ↔ ψ ∈ Ω₂.1) : (∼φ ∈ Ω₁.1) ↔ (∼ψ ∈ Ω₂.1) := ⟨neg_imp $ h.mpr, neg_imp $ h.mp⟩
+
+lemma iff_mem_conj : (⋀Γ ∈ Ω) ↔ (∀ φ ∈ Γ, φ ∈ Ω) := by simp [membership_iff, iff_provable_list_conj];
 
 -- These lemmata require H normality
 section Normal
 
-variable [H.IsNormal]
+variable [System.K H]
 
-lemma iff_mem_multibox : (□^[n]φ ∈ Ω.theory) ↔ (∀ {Ω' : MCT H}, (□''⁻¹^[n]Ω.theory ⊆ Ω'.theory) → (φ ∈ Ω'.theory)) := by
+lemma iff_mem_multibox : (□^[n]φ ∈ Ω) ↔ (∀ {Ω' : MCS H}, (□''⁻¹^[n]Ω.1 ⊆ Ω'.1) → (φ ∈ Ω')) := by
   constructor;
   . intro hp Ω' hΩ'; apply hΩ'; simpa;
   . contrapose;
     push_neg;
     intro hp;
-    obtain ⟨Ω', hΩ'⟩ := lindenbaum (H := H) (T := insert (∼φ) (□''⁻¹^[n]Ω.theory)) (by
+    obtain ⟨Ω', hΩ'⟩ := lindenbaum (H := H) (T := insert (∼φ) (□''⁻¹^[n]Ω.1)) (by
       apply unprovable_iff_insert_neg_consistent.mp;
       by_contra hC;
       obtain ⟨Γ, hΓ₁, hΓ₂⟩ := Context.provable_iff.mp hC;
@@ -495,16 +497,16 @@ lemma iff_mem_multibox : (□^[n]φ ∈ Ω.theory) ↔ (∀ {Ω' : MCT H}, (□'
     . apply iff_mem_neg.mp;
       apply hΩ';
       simp only [Set.mem_insert_iff, true_or]
-lemma iff_mem_box : (□φ ∈ Ω.theory) ↔ (∀ {Ω' : MCT H}, (□''⁻¹Ω.theory ⊆ Ω'.theory) → (φ ∈ Ω'.theory)) := iff_mem_multibox (n := 1)
+lemma iff_mem_box : (□φ ∈ Ω) ↔ (∀ {Ω' : MCS H}, (□''⁻¹Ω.1 ⊆ Ω'.1) → (φ ∈ Ω'.1)) := iff_mem_multibox (n := 1)
 
-lemma multibox_dn_iff : (□^[n](∼∼φ) ∈ Ω.theory) ↔ (□^[n]φ ∈ Ω.theory) := by
+lemma multibox_dn_iff : (□^[n](∼∼φ) ∈ Ω) ↔ (□^[n]φ ∈ Ω) := by
   simp only [iff_mem_multibox];
   constructor;
   . intro h Ω hΩ; exact iff_mem_negneg.mp $ h hΩ;
   . intro h Ω hΩ; exact iff_mem_negneg.mpr $ h hΩ;
-lemma box_dn_iff : (□(∼∼φ) ∈ Ω.theory) ↔ (□φ ∈ Ω.theory) := multibox_dn_iff (n := 1)
+lemma box_dn_iff : (□(∼∼φ) ∈ Ω) ↔ (□φ ∈ Ω) := multibox_dn_iff (n := 1)
 
-lemma mem_multibox_dual : □^[n]φ ∈ Ω.theory ↔ ∼(◇^[n](∼φ)) ∈ Ω.theory := by
+lemma mem_multibox_dual : □^[n]φ ∈ Ω ↔ ∼(◇^[n](∼φ)) ∈ Ω := by
   simp only [membership_iff];
   constructor;
   . intro h;
@@ -521,13 +523,13 @@ lemma mem_multibox_dual : □^[n]φ ∈ Ω.theory ↔ ∼(◇^[n](∼φ)) ∈ Ω
     constructor;
     . assumption;
     . exact FiniteContext.provable_iff.mpr $ imp_trans''! (FiniteContext.provable_iff.mp hΓ₂) (and₂'! multibox_duality!);
-lemma mem_box_dual : □φ ∈ Ω.theory ↔ (∼(◇(∼φ)) ∈ Ω.theory) := mem_multibox_dual (n := 1)
+lemma mem_box_dual : □φ ∈ Ω ↔ (∼(◇(∼φ)) ∈ Ω) := mem_multibox_dual (n := 1)
 
--- lemma multidia_dn_iff : (◇^[n](∼∼φ) ∈ Ω.theory) ↔ (◇^[n]φ ∈ Ω.theory) := by sorry
+-- lemma multidia_dn_iff : (◇^[n](∼∼φ) ∈ Ω) ↔ (◇^[n]φ ∈ Ω) := by sorry
 
--- lemma dia_dn_iff : (◇(∼∼φ) ∈ Ω.theory) ↔ (◇φ) ∈ Ω.theory := neg_iff box_dn_iff -- TODO: multidia_dn_iff (n := 1)
+-- lemma dia_dn_iff : (◇(∼∼φ) ∈ Ω) ↔ (◇φ) ∈ Ω := neg_iff box_dn_iff -- TODO: multidia_dn_iff (n := 1)
 
-lemma mem_multidia_dual : ◇^[n]φ ∈ Ω.theory ↔ ∼(□^[n](∼φ)) ∈ Ω.theory := by
+lemma mem_multidia_dual : ◇^[n]φ ∈ Ω ↔ ∼(□^[n](∼φ)) ∈ Ω := by
   simp only [membership_iff];
   constructor;
   . intro h;
@@ -544,9 +546,9 @@ lemma mem_multidia_dual : ◇^[n]φ ∈ Ω.theory ↔ ∼(□^[n](∼φ)) ∈ Ω
     constructor;
     . assumption;
     . exact FiniteContext.provable_iff.mpr $ imp_trans''! (FiniteContext.provable_iff.mp hΓ₂) (and₂'! multidia_duality!);
-lemma mem_dia_dual : ◇φ ∈ Ω.theory ↔ (∼(□(∼φ)) ∈ Ω.theory) := mem_multidia_dual (n := 1)
+lemma mem_dia_dual : ◇φ ∈ Ω ↔ (∼(□(∼φ)) ∈ Ω) := mem_multidia_dual (n := 1)
 
-lemma iff_mem_multidia : (◇^[n]φ ∈ Ω.theory) ↔ (∃ Ω' : MCT H, (□''⁻¹^[n]Ω.theory ⊆ Ω'.theory) ∧ (φ ∈ Ω'.theory)) := by
+lemma iff_mem_multidia : (◇^[n]φ ∈ Ω) ↔ (∃ Ω' : MCS H, (□''⁻¹^[n]Ω.1 ⊆ Ω'.1) ∧ (φ ∈ Ω'.1)) := by
   constructor;
   . intro h;
     have := mem_multidia_dual.mp h;
@@ -567,9 +569,9 @@ lemma iff_mem_multidia : (◇^[n]φ ∈ Ω.theory) ↔ (∃ Ω' : MCT H, (□''�
     constructor;
     . exact h₁;
     . exact iff_mem_neg.mp $ mem_dn_iff.mp h₂;
-lemma iff_mem_dia : (◇φ ∈ Ω.theory) ↔ (∃ Ω' : MCT H, (□''⁻¹Ω.theory ⊆ Ω'.theory) ∧ (φ ∈ Ω'.theory)) := iff_mem_multidia (n := 1)
+lemma iff_mem_dia : (◇φ ∈ Ω) ↔ (∃ Ω' : MCS H, (□''⁻¹Ω.1 ⊆ Ω'.1) ∧ (φ ∈ Ω'.1)) := iff_mem_multidia (n := 1)
 
-lemma multibox_multidia : (∀ {φ : Formula α}, (□^[n]φ ∈ Ω₁.theory → φ ∈ Ω₂.theory)) ↔ (∀ {φ : Formula α}, (φ ∈ Ω₂.theory → ◇^[n]φ ∈ Ω₁.theory)) := by
+lemma multibox_multidia : (∀ {φ : Formula α}, (□^[n]φ ∈ Ω₁.1 → φ ∈ Ω₂.1)) ↔ (∀ {φ : Formula α}, (φ ∈ Ω₂.1 → ◇^[n]φ ∈ Ω₁.1)) := by
   constructor;
   . intro H φ;
     contrapose;
@@ -590,21 +592,19 @@ lemma multibox_multidia : (∀ {φ : Formula α}, (□^[n]φ ∈ Ω₁.theory �
 
 variable {Γ : List (Formula α)}
 
-omit [H.IsNormal] in
-lemma iff_mem_conj : (⋀Γ ∈ Ω.theory) ↔ (∀ φ ∈ Γ, φ ∈ Ω.theory) := by simp [membership_iff, iff_provable_list_conj];
-
-lemma iff_mem_multibox_conj : (□^[n]⋀Γ ∈ Ω.theory) ↔ (∀ φ ∈ Γ, □^[n]φ ∈ Ω.theory) := by
+lemma iff_mem_multibox_conj : (□^[n]⋀Γ ∈ Ω) ↔ (∀ φ ∈ Γ, □^[n]φ ∈ Ω) := by
   simp only [iff_mem_multibox, iff_mem_conj];
   constructor;
-  . intro h φ hp Ω' hΩ';
-    exact (h hΩ') φ hp;
-  . intro h Ω' hΩ' φ hp;
-    exact @h φ hp Ω' hΩ';
+  . intro h φ hφ Ω' hΩ';
+    exact h hΩ' _ hφ;
+  . intro h Ω' hΩ' φ hφ;
+    apply h _ hφ;
+    tauto;
 
-lemma iff_mem_box_conj : (□⋀Γ ∈ Ω.theory) ↔ (∀ φ ∈ Γ, □φ ∈ Ω.theory) := iff_mem_multibox_conj (n := 1)
+lemma iff_mem_box_conj : (□⋀Γ ∈ Ω) ↔ (∀ φ ∈ Γ, □φ ∈ Ω) := iff_mem_multibox_conj (n := 1)
 
 end Normal
 
-end MaximalConsistentFormulaSet
+end MaximalConsistentSet
 
 end LO.Modal
