Foundation/Modal/Complement.lean
@@ -1,0 +1,89 @@
+import Foundation.Modal.Formula
+import Foundation.Modal.Subformulas
+
+
+namespace LO.Modal
+
+
+namespace Formula
+
+def complement : Formula α → Formula α
+  | ∼φ => φ
+  | φ  => ∼φ
+prefix:80 "-" => complement
+
+namespace complement
+
+variable {φ ψ : Formula α}
+
+@[simp] lemma neg_def : -(∼φ) = φ := by
+  induction φ using Formula.rec' <;> simp_all [complement]
+
+@[simp] lemma bot_def : -(⊥ : Formula α) = ∼(⊥) := by simp only [complement, imp_inj, and_true]; rfl;
+
+@[simp] lemma box_def : -(□φ) = ∼(□φ) := by simp only [complement, imp_inj, and_true]; rfl;
+
+lemma imp_def₁ (hq : ψ ≠ ⊥) : -(φ ➝ ψ) = ∼(φ ➝ ψ) := by
+  simp only [complement];
+  split;
+  . rename_i h; simp [imp_eq, falsum_eq, hq] at h;
+  . rfl;
+
+lemma imp_def₂ (hq : ψ = ⊥) : -(φ ➝ ψ) = φ := by
+  subst_vars;
+  apply neg_def;
+
+lemma resort_box (h : -φ = □ψ) : φ = ∼□ψ := by
+  simp [complement] at h;
+  split at h;
+  . subst_vars; rfl;
+  . contradiction;
+
+lemma or [DecidableEq α] (φ : Formula α) : -φ = ∼φ ∨ ∃ ψ, ∼ψ = φ := by
+  induction φ using Formula.cases_neg with
+  | himp _ _ hn => simp [imp_def₁ hn];
+  | hfalsum => simp;
+  | hneg => simp;
+  | hatom a => simp [complement];
+  | hbox φ => simp [complement]; rfl;
+
+end complement
+
+end Formula
+
+
+namespace FormulaFinset
+
+variable [DecidableEq α]
+
+def complementary (P : FormulaFinset α) : FormulaFinset α := P ∪ (P.image (Formula.complement))
+postfix:80 "⁻" => complementary
+
+variable {P P₁ P₂ : FormulaFinset α} {φ ψ χ : Formula α}
+
+lemma complementary_mem (h : φ ∈ P) : φ ∈ P⁻ := by simp_all [complementary];
+
+lemma complementary_comp (h : φ ∈ P) : -φ ∈ P⁻ := by simp [complementary]; tauto;
+
+lemma complementary_mem_box (hi : ∀ {ψ χ}, ψ ➝ χ ∈ P → ψ ∈ P := by trivial) : □φ ∈ P⁻ → □φ ∈ P := by
+  intro h;
+  simp [complementary] at h;
+  rcases h with (h | ⟨ψ, hq, eq⟩);
+  . assumption;
+  . replace eq := Formula.complement.resort_box eq;
+    subst eq;
+    exact hi hq;
+
+
+
+class ComplementaryClosed (P : FormulaFinset α) (S : FormulaFinset α) : Prop where
+  subset : P ⊆ S⁻
+  either : ∀ φ ∈ S, φ ∈ P ∨ -φ ∈ P
+
+
+def SubformulaeComplementaryClosed (P : FormulaFinset α) (φ : Formula α) : Prop := P.ComplementaryClosed φ.subformulas
+
+
+end FormulaFinset
+
+end LO.Modal
