Foundation/Modal/Hilbert2/Basic.lean
@@ -1,0 +1,112 @@
+import Foundation.Modal.Formula
+import Foundation.Modal.Substitution
+import Foundation.Modal.System.K
+import Foundation.Logic.HilbertStyle.Lukasiewicz
+
+namespace LO.Modal
+
+open System
+
+variable {α : Type*}
+
+structure Hilbert (α : Type*) where
+  axioms : Set (Formula α)
+
+class Hilbert.FiniteAxiomatizable (H : Hilbert α) where
+  axioms_fin : Set.Finite H.axioms
+
+variable {H H₁ H₂ : Hilbert α}
+
+inductive Hilbert.Deduction (H : Hilbert α) : (Formula α) → Type _
+  | maxm {φ}      : φ ∈ H.axioms → Deduction H φ
+  | mdp {φ ψ}     : Deduction H (φ ➝ ψ) → Deduction H φ → Deduction H ψ
+  | subst {φ} (s) : Deduction H φ → Deduction H (φ⟦s⟧)
+  | nec {φ}       : Deduction H φ → Deduction H (□φ)
+  | imply₁ φ ψ    : Deduction H $ Axioms.Imply₁ φ ψ
+  | imply₂ φ ψ χ  : Deduction H $ Axioms.Imply₂ φ ψ χ
+  | ec φ ψ        : Deduction H $ Axioms.ElimContra φ ψ
+
+namespace Hilbert.Deduction
+
+instance : System (Formula α) (Hilbert α) := ⟨Deduction⟩
+
+instance : System.Lukasiewicz H where
+  mdp := mdp
+  imply₁ := imply₁
+  imply₂ := imply₂
+  elim_contra := ec
+
+instance : System.Classical H where
+
+instance : System.HasDiaDuality H := inferInstance
+
+instance : System.Necessitation H := ⟨nec⟩
+
+lemma maxm! {φ} (h : φ ∈ H.axioms) : H ⊢! φ := ⟨maxm h⟩
+
+lemma subst! {φ} (s) (h : H ⊢! φ) : H ⊢! φ⟦s⟧ := ⟨subst s h.some⟩
+
+end Hilbert.Deduction
+
+
+namespace Hilbert
+
+open Deduction
+
+namespace Deduction
+
+variable {H : Hilbert α}
+
+noncomputable def inducition!
+  {motive      : (φ : Formula α) → H ⊢! φ → Sort*}
+  (hMaxm       : ∀ {φ}, (h : φ ∈ H.axioms) → motive φ ⟨maxm h⟩)
+  (hMdp        : ∀ {φ ψ}, {hpq : H ⊢! φ ➝ ψ} → {hp : H ⊢! φ} → motive (φ ➝ ψ) hpq → motive φ hp → motive ψ (mdp! hpq hp))
+  (hNec        : ∀ {φ}, {hp : H ⊢! φ} → (ihp : motive φ hp) → motive (□φ) (nec! hp))
+  (hSubst      : ∀ {φ} (s : Substitution α), {hp : H ⊢! φ} → (ihp : motive φ hp) → motive (φ⟦s⟧) (subst! s hp))
+  (hImply₁     : ∀ {φ ψ}, motive (φ ➝ ψ ➝ φ) $ ⟨imply₁ φ ψ⟩)
+  (hImply₂     : ∀ {φ ψ χ}, motive ((φ ➝ ψ ➝ χ) ➝ (φ ➝ ψ) ➝ φ ➝ χ) $ ⟨imply₂ φ ψ χ⟩)
+  (hElimContra : ∀ {φ ψ}, motive (Axioms.ElimContra φ ψ) $ ⟨ec φ ψ⟩)
+  : ∀ {φ}, (d : H ⊢! φ) → motive φ d := by
+  intro φ d;
+  induction d.some with
+  | maxm h => exact hMaxm h
+  | mdp hpq hp ihpq ihp => exact hMdp (ihpq ⟨hpq⟩) (ihp ⟨hp⟩)
+  | nec hp ih => exact hNec (ih ⟨hp⟩)
+  | subst s hp ih => exact hSubst s (ih ⟨hp⟩)
+  | _ => aesop;
+
+end Deduction
+
+
+variable {H H₁ H₂ : Hilbert α}
+
+abbrev theorems (H : Hilbert α) := System.theory H
+
+lemma of_subset (hs : H₁.axioms ⊆ H₂.axioms) : H₁ ⊢! φ → H₂ ⊢! φ := by
+  intro h;
+  induction h using Deduction.inducition! with
+  | hMaxm h => exact maxm! $ hs h;
+  | hMdp ih₁ ih₂ => exact mdp! ih₁ ih₂;
+  | hNec ih => exact nec! ih;
+  | hSubst s ih => exact subst! s ih;
+  | _ => simp;
+
+lemma weakerThan_of_dominate_axioms (hMaxm : ∀ {φ : Formula α}, φ ∈ H₁.axioms → H₂ ⊢! φ) : H₁ ≤ₛ H₂ := by
+  apply System.weakerThan_iff.mpr;
+  intro φ h;
+  induction h using Deduction.inducition! with
+  | hMaxm h => exact hMaxm h;
+  | hMdp ih₁ ih₂ => exact mdp! ih₁ ih₂;
+  | hNec ih => exact nec! ih;
+  | hSubst s ih => exact subst! s ih;
+  | _ => simp;
+
+lemma weakerThan_of_subset_axioms (hSubset : H₁.axioms ⊆ H₂.axioms) : H₁ ≤ₛ H₂ := by
+  apply weakerThan_of_dominate_axioms;
+  intro φ hp;
+  exact ⟨Deduction.maxm $ hSubset hp⟩;
+
+end Hilbert
+
+
+end LO.Modal
