Foundation/Modal/Hilbert2/Geach.lean
@@ -1,0 +1,56 @@
+import Foundation.Modal.Hilbert2.WellKnown
+
+namespace LO.Modal
+
+namespace Hilbert
+
+variable (α) [DecidableEq α] [h2 : HasElements 2 α]
+
+protected def Geach (G : Set (GeachConfluent.Taple)) : Hilbert α := ⟨
+  {Axioms.K (.atom (h2.vec[0])) (.atom (h2.vec[1]))}
+  ∪ G.image (λ t => Axioms.Geach t (h2.vec[0]))
+⟩
+
+instance HasT_of_mem_0_0_1_0 (h : ⟨0, 0, 1, 0⟩ ∈ G) : HasT (Hilbert.Geach α G) where
+  p := h2.vec[0]
+  mem_T := by
+    unfold Hilbert.Geach;
+    simp;
+    use ⟨0, 0, 1, 0⟩;
+    simpa;
+
+instance HasB_of_mem_0_1_0_1 (h : ⟨0, 1, 0, 1⟩ ∈ G) : HasB (Hilbert.Geach α G) where
+  p := h2.vec[0]
+  mem_B := by
+    unfold Hilbert.Geach;
+    simp;
+    use ⟨0, 1, 0, 1⟩;
+    simpa;
+
+instance HasD_of_mem_0_0_1_1 (h : ⟨0, 0, 1, 1⟩ ∈ G) : HasD (Hilbert.Geach α G) where
+  p := h2.vec[0]
+  mem_D := by
+    unfold Hilbert.Geach;
+    simp;
+    use ⟨0, 0, 1, 1⟩;
+    simpa;
+
+instance HasFour_of_mem_0_2_1_0 (h : ⟨0, 2, 1, 0⟩ ∈ G) : HasFour (Hilbert.Geach α G) where
+  p := h2.vec[0]
+  mem_Four := by
+    unfold Hilbert.Geach;
+    simp;
+    use ⟨0, 2, 1, 0⟩;
+    simpa;
+
+instance HasFive_of_mem_1_1_0_1 (h : ⟨1, 1, 0, 1⟩ ∈ G) : HasFive (Hilbert.Geach α G) where
+  p := h2.vec[0]
+  mem_Five := by
+    unfold Hilbert.Geach;
+    simp;
+    use ⟨1, 1, 0, 1⟩;
+    simpa;
+
+end Hilbert
+
+end LO.Modal
