Foundation/Modal/Hilbert2/K.lean
@@ -1,0 +1,40 @@
+import Foundation.Modal.Hilbert2.Basic
+import Foundation.Vorspiel.HasElements
+
+namespace LO.Modal.Hilbert
+
+variable {H : Hilbert α}
+
+open Deduction
+
+section
+
+class HasK (H : Hilbert α) where
+  p : α
+  q : α
+  ne_pq : p ≠ q
+  mem_K : Axioms.K (.atom p) (.atom q) ∈ H.axioms := by tauto;
+
+instance [DecidableEq α] [hK : H.HasK] : System.HasAxiomK H where
+  K φ ψ := by
+    simpa [hK.ne_pq] using
+      subst (s := λ b => if hK.p = b then φ else if hK.q = b then ψ else (.atom b)) $
+      maxm hK.mem_K;
+
+end
+
+
+section
+
+protected def K : Hilbert ℕ := ⟨{Axioms.K (.atom 0) (.atom 1)}⟩
+
+instance : (Hilbert.K).HasK where
+  p := 0
+  q := 1
+  ne_pq := by trivial;
+
+instance : System.K (Hilbert.K) where
+
+end
+
+end LO.Modal.Hilbert
