Foundation/Modal/Hilbert2/Maximal/Unprovability.lean
@@ -1,0 +1,92 @@
+import Foundation.Modal.Hilbert2.Maximal.Basic
+import Foundation.IntProp.Kripke.Classical
+
+namespace LO.Modal
+
+open System
+
+open IntProp
+
+open Hilbert
+open Hilbert.Deduction
+open Formula
+
+namespace Hilbert
+
+
+namespace Triv
+
+lemma unprovable_AxiomL : Hilbert.Triv ⊬ (Axioms.L (.atom a)) := by
+  apply Hilbert.Triv.classical_reducible.not.mpr;
+  apply IntProp.Hilbert.Cl.unprovable_of_exists_classicalValuation;
+  use (λ _ => False);
+  simp [Axioms.L, TrivTranslation, toPropFormula, IntProp.Formula.Kripke.Satisfies];
+
+end Triv
+
+
+namespace Ver
+
+lemma unprovable_AxiomP : (Hilbert.Ver) ⊬ Axioms.P := by
+  apply Hilbert.Ver.classical_reducible.not.mpr;
+  apply IntProp.Hilbert.Cl.unprovable_of_exists_classicalValuation;
+  dsimp [VerTranslation, toPropFormula, IntProp.Formula.Kripke.Satisfies];
+  use (λ _ => True);
+  simp;
+
+end Ver
+
+
+namespace K4
+
+lemma provable_Cl_trivTranslated : (Hilbert.K4) ⊢! φ → (Hilbert.Cl _) ⊢! φᵀᴾ := by
+  intro h;
+  apply Hilbert.Triv.classical_reducible.mp;
+  exact System.weakerThan_iff.mp (by simp) h;
+
+lemma unprovable_AxiomL : Hilbert.K4 ⊬ (Axioms.L (.atom a)) := by
+  apply not_imp_not.mpr provable_Cl_trivTranslated;
+  apply IntProp.Hilbert.Cl.unprovable_of_exists_classicalValuation;
+  use (λ _ => False);
+  simp [Axioms.L, TrivTranslation, toPropFormula, IntProp.Formula.Kripke.Satisfies];
+
+end K4
+
+
+namespace GL
+
+lemma provable_CL_verTranslated : (Hilbert.GL) ⊢! φ → (Hilbert.Cl _) ⊢! φⱽᴾ := by
+  intro h;
+  induction h using Deduction.inducition! with
+    | hMaxm a =>
+      rcases a with (⟨_, _, rfl⟩ | ⟨_, rfl⟩) <;> simp [VerTranslation, toPropFormula];
+    | hMdp ih₁ ih₂ =>
+      dsimp [VerTranslation] at ih₁ ih₂;
+      exact ih₁ ⨀ ih₂;
+    | hSubst s ih => sorry;
+    | _ => simp [VerTranslation, toPropFormula];
+
+lemma unprovable_AxiomT : (Hilbert.GL) ⊬ Axioms.T (.atom a) := by
+  apply not_imp_not.mpr provable_CL_verTranslated;
+  apply IntProp.Hilbert.Cl.unprovable_of_exists_classicalValuation;
+  use (λ _ => False);
+  simp [Axioms.T, VerTranslation, toPropFormula, IntProp.Formula.Kripke.Satisfies];
+
+instance : System.Consistent (Hilbert.GL) := by
+  apply consistent_iff_exists_unprovable.mpr;
+  use (Axioms.T (atom 0));
+  apply unprovable_AxiomT;
+
+end GL
+
+theorem not_S4_weakerThan_GL : ¬(Hilbert.S4) ≤ₛ (Hilbert.GL) := by
+  apply System.not_weakerThan_iff.mpr;
+  existsi (Axioms.T (atom 0));
+  constructor;
+  . exact axiomT!;
+  . exact GL.unprovable_AxiomT;
+
+end Hilbert
+
+
+end LO.Modal
