Foundation/Modal/Hilbert2/WellKnown.lean
@@ -1,0 +1,167 @@
+import Foundation.Modal.Hilbert2.K
+
+namespace LO.Modal
+
+namespace Hilbert
+
+section
+
+open Deduction
+
+variable {H : Hilbert α}
+variable [DecidableEq α]
+
+
+class HasT (H : Hilbert α) where
+  p : α
+  mem_T : Axioms.T (.atom p) ∈ H.axioms := by tauto;
+
+instance [hT : H.HasT] : System.HasAxiomT H where
+  T φ := by simpa using subst (s := λ b => if hT.p = b then φ else (.atom b)) $ maxm hT.mem_T;
+
+
+class HasB (H : Hilbert α) where
+  p : α
+  mem_B : Axioms.B (.atom p) ∈ H.axioms := by tauto;
+
+instance [hB : H.HasB] : System.HasAxiomB H where
+  B φ := by simpa using subst (s := λ b => if hB.p = b then φ else (.atom b)) $ maxm hB.mem_B;
+
+
+class HasD (H : Hilbert α) where
+  p : α
+  mem_D : Axioms.D (.atom p) ∈ H.axioms := by tauto;
+
+instance [hD : H.HasD] : System.HasAxiomD H where
+  D φ := by simpa using subst (s := λ b => if hD.p = b then φ else (.atom b)) $ maxm hD.mem_D;
+
+
+class HasFour (H : Hilbert α) where
+  p : α
+  mem_Four : Axioms.Four (.atom p) ∈ H.axioms := by tauto;
+
+instance [hFour : H.HasFour] : System.HasAxiomFour H where
+  Four φ := by simpa using subst (s := λ b => if hFour.p = b then φ else (.atom b)) $ maxm hFour.mem_Four;
+
+
+class HasFive (H : Hilbert α) where
+  p : α
+  mem_Five : Axioms.Five (.atom p) ∈ H.axioms := by tauto;
+
+instance [hFive : H.HasFive] : System.HasAxiomFive H where
+  Five φ := by simpa using subst (s := λ b => if hFive.p = b then φ else (.atom b)) $ maxm hFive.mem_Five;
+
+
+class HasDot2 (H : Hilbert α) where
+  p : α
+  mem_Dot2 : Axioms.Dot2 (.atom p) ∈ H.axioms := by tauto;
+
+instance [hDot2 : H.HasDot2] : System.HasAxiomDot2 H where
+  Dot2 φ := by simpa using subst (s := λ b => if hDot2.p = b then φ else (.atom b)) $ maxm hDot2.mem_Dot2;
+
+
+class HasDot3 (H : Hilbert α) where
+  p : α
+  q : α
+  ne_pq : p ≠ q
+  mem_Dot3 : Axioms.Dot3 (.atom p) (.atom q) ∈ H.axioms := by tauto;
+
+instance [hDot3 : H.HasDot3] : System.HasAxiomDot3 H where
+  Dot3 φ ψ := by
+    simpa [hDot3.ne_pq] using
+      subst (s := λ b => if hDot3.p = b then φ else if hDot3.q = b then ψ else (.atom b)) $
+      maxm hDot3.mem_Dot3;
+
+
+class HasL (H : Hilbert α) where
+  p : α
+  mem_L : Axioms.L (.atom p) ∈ H.axioms := by tauto;
+
+instance [hL : H.HasL] : System.HasAxiomL H where
+  L φ := by simpa using subst (s := λ b => if hL.p = b then φ else (.atom b)) $ maxm hL.mem_L;
+
+
+class HasGrz (H : Hilbert α) where
+  p : α
+  mem_Grz : Axioms.Grz (.atom p) ∈ H.axioms := by tauto;
+
+instance [hGrz : H.HasGrz] : System.HasAxiomGrz H where
+  Grz φ := by simpa using subst (s := λ b => if hGrz.p = b then φ else (.atom b)) $ maxm hGrz.mem_Grz;
+
+
+class HasTc (H : Hilbert α) where
+  p : α
+  mem_Tc : Axioms.Tc (.atom p) ∈ H.axioms := by tauto;
+
+instance [hTc : H.HasTc] : System.HasAxiomTc H where
+  Tc φ := by simpa using subst (s := λ b => if hTc.p = b then φ else (.atom b)) $ maxm hTc.mem_Tc;
+
+
+class HasVer (H : Hilbert α) where
+  p : α
+  mem_Ver : Axioms.Ver (.atom p) ∈ H.axioms := by tauto;
+
+instance [DecidableEq α] [hVer : H.HasVer] : System.HasAxiomVer H where
+  Ver φ := by simpa using subst (s := λ b => if hVer.p = b then φ else (.atom b)) $ maxm hVer.mem_Ver;
+
+end
+
+
+protected abbrev Ver : Hilbert ℕ := ⟨{Axioms.K (.atom 0) (.atom 1), Axioms.Ver (.atom 0)}⟩
+instance : (Hilbert.Ver).HasK where p := 0; q := 1; ne_pq := by trivial
+instance : (Hilbert.Ver).HasVer where p := 0
+
+
+protected abbrev Triv : Hilbert ℕ := ⟨{ Axioms.K (.atom 0) (.atom 1), Axioms.T (.atom 0), Axioms.Tc (.atom 0)}⟩
+instance : (Hilbert.Triv).HasK where p := 0; q := 1; ne_pq := by trivial;
+instance : (Hilbert.Triv).HasT where p := 0
+instance : (Hilbert.Triv).HasTc where p := 0
+
+
+protected abbrev K4 : Hilbert ℕ := ⟨{Axioms.K (.atom 0) (.atom 1), Axioms.Four (.atom 0)}⟩
+instance : (Hilbert.K4).HasK where p := 0; q := 1; ne_pq := by trivial
+instance : (Hilbert.K4).HasFour where p := 0
+
+
+protected abbrev S4 : Hilbert ℕ := ⟨{Axioms.K (.atom 0) (.atom 1), Axioms.T (.atom 0), Axioms.Four (.atom 0)}⟩
+instance : (Hilbert.S4).HasK where p := 0; q := 1; ne_pq := by trivial
+instance : (Hilbert.S4).HasT where p := 0
+instance : (Hilbert.S4).HasFour where p := 0
+
+
+protected abbrev S4Dot2 : Hilbert ℕ := ⟨{Axioms.K (.atom 0) (.atom 1), Axioms.T (.atom 0), Axioms.Four (.atom 0), Axioms.Dot2 (.atom 0)}⟩
+instance : (Hilbert.S4Dot2).HasK where p := 0; q := 1; ne_pq := by trivial
+instance : (Hilbert.S4Dot2).HasT where p := 0
+instance : (Hilbert.S4Dot2).HasFour where p := 0
+instance : (Hilbert.S4Dot2).HasDot2 where p := 0
+
+
+protected abbrev S4Dot3 : Hilbert ℕ := ⟨{Axioms.K (.atom 0) (.atom 1), Axioms.T (.atom 0), Axioms.Four (.atom 0), Axioms.Dot3 (.atom 0) (.atom 1)}⟩
+instance : (Hilbert.S4Dot3).HasK where p := 0; q := 1; ne_pq := by trivial
+instance : (Hilbert.S4Dot3).HasT where p := 0
+instance : (Hilbert.S4Dot3).HasFour where p := 0
+instance : (Hilbert.S4Dot3).HasDot3 where p := 0; q := 1; ne_pq := by trivial
+
+
+protected abbrev S5 : Hilbert ℕ := ⟨{Axioms.K (.atom 0) (.atom 1), Axioms.T (.atom 0), Axioms.Five (.atom 0)}⟩
+instance : (Hilbert.S5).HasK where p := 0; q := 1; ne_pq := by trivial
+instance : (Hilbert.S5).HasT where p := 0
+instance : (Hilbert.S5).HasFive where p := 0
+
+
+protected abbrev GL : Hilbert ℕ := ⟨{Axioms.K (.atom 0) (.atom 1), Axioms.L (.atom 0)}⟩
+instance : (Hilbert.GL).HasK where p := 0; q := 1; ne_pq := by trivial
+instance : (Hilbert.GL).HasL where p := 0
+
+
+protected abbrev Grz : Hilbert ℕ := ⟨{Axioms.K (.atom 0) (.atom 1), Axioms.Grz (.atom 0)}⟩
+instance : (Hilbert.Grz).HasK where p := 0; q := 1; ne_pq := by trivial
+instance : (Hilbert.Grz).HasGrz where p := 0
+
+
+@[simp] lemma K4_weakerThan_Triv : Hilbert.K4 ≤ₛ Hilbert.Triv := weakerThan_of_dominate_axioms $ by simp;
+
+
+end Hilbert
+
+end LO.Modal
