Foundation/Modal/Subformulas.lean
@@ -1,0 +1,104 @@
+import Foundation.Modal.Formula
+
+
+namespace LO.Modal
+
+def Formula.subformulas [DecidableEq α] : Formula α → FormulaFinset α
+  | atom a => {(atom a)}
+  | ⊥      => {⊥}
+  | φ ➝ ψ  => insert (φ ➝ ψ) (φ.subformulas ∪ ψ.subformulas)
+  | □φ     => insert (□φ) φ.subformulas
+
+namespace Formula.subformulas
+
+variable [DecidableEq α]
+
+@[simp] lemma mem_self {φ : Formula α} : φ ∈ φ.subformulas := by induction φ <;> { simp [subformulas]; try tauto; }
+
+variable {φ ψ χ : Formula α}
+
+lemma mem_imp (h : (ψ ➝ χ) ∈ φ.subformulas) : ψ ∈ φ.subformulas ∧ χ ∈ φ.subformulas := by
+  induction φ using Formula.rec' with
+  | himp => simp_all [subformulas]; rcases h with ⟨_⟩ | ⟨⟨_⟩ | ⟨_⟩⟩ <;> simp_all
+  | _ => simp_all [subformulas];
+
+lemma mem_imp₁ (h : (ψ ➝ χ) ∈ φ.subformulas) : ψ ∈ φ.subformulas := mem_imp h |>.1
+
+lemma mem_imp₂ (h : (ψ ➝ χ) ∈ φ.subformulas) : χ ∈ φ.subformulas := mem_imp h |>.2
+
+lemma mem_box (h : □ψ ∈ φ.subformulas) : ψ ∈ φ.subformulas := by
+  induction φ using Formula.rec' <;> {
+    simp_all [subformulas];
+    try rcases h with (hq | hr); simp_all; simp_all;
+  };
+
+-- TODO: add tactic like `subformulas`.
+attribute [aesop safe 5 forward]
+  mem_imp₁
+  mem_imp₂
+  mem_box
+
+@[simp]
+lemma complexity_lower (h : ψ ∈ φ.subformulas) : ψ.complexity ≤ φ.complexity  := by
+  induction φ using Formula.rec' with
+  | himp φ₁ φ₂ ihp₁ ihp₂ =>
+    simp_all [subformulas];
+    rcases h with _ | h₁ | h₂;
+    . subst_vars; simp [Formula.complexity];
+    . have := ihp₁ h₁; simp [Formula.complexity]; omega;
+    . have := ihp₂ h₂; simp [Formula.complexity]; omega;
+  | hbox φ ihp =>
+    simp_all [subformulas];
+    rcases h with _ | h₁;
+    . subst_vars; simp [Formula.complexity];
+    . have := ihp h₁; simp [Formula.complexity]; omega;
+  | hatom => simp_all [subformulas];
+  | hfalsum => simp_all [subformulas, Formula.complexity];
+
+/-
+@[simp]
+lemma degree_lower (h : ψ ∈ φ.subformulas) : ψ.degree ≤ φ.degree := by
+  induction φ using Formula.rec' with
+  | himp φ₁ φ₂ ihp₁ ihp₂ =>
+    simp_all [subformulas];
+    rcases h with rfl | h₁ | h₂;
+    . simp_all [Formula.degree];
+    . have := ihp₁ h₁; simp [Formula.degree]; omega;
+    . have := ihp₂ h₂; simp [Formula.degree]; omega;
+  | hbox φ ihp =>
+    simp_all [subformulae];
+    rcases h with _ | h₁;
+    . subst_vars; simp [Formula.degree];
+    . have := ihp h₁; simp [Formula.degree]; omega;
+  | hatom =>
+    simp_all [subformulae];
+    rcases h with rfl | rfl <;> simp [Formula.degree];
+  | hfalsum => simp_all [subformulae, Formula.degree];
+-/
+
+end Formula.subformulas
+
+
+class FormulaSet.SubformulaClosed (P : FormulaSet α) where
+  imp_closed : ∀ {φ ψ}, φ ➝ ψ ∈ P → φ ∈ P ∧ ψ ∈ P
+  box_closed : ∀ {φ}, □φ ∈ P → φ ∈ P
+
+namespace FormulaSet.SubformulaClosed
+
+variable {φ : Formula α} {P : FormulaSet α} [hP : P.SubformulaClosed]
+
+lemma mem_imp₁ (h : φ ➝ ψ ∈ P) : φ ∈ P := hP.imp_closed h |>.1
+lemma mem_imp₂ (h : φ ➝ ψ ∈ P) : ψ ∈ P := hP.imp_closed h |>.2
+lemma mem_box (h : □φ ∈ P) : φ ∈ P := hP.box_closed h
+
+instance {φ : Formula α} [DecidableEq α] : FormulaSet.SubformulaClosed (φ.subformulas).toSet where
+  box_closed := by
+    intro φ hφ;
+    exact Formula.subformulas.mem_box hφ;
+  imp_closed := by
+    intro φ ψ hφ;
+    exact Formula.subformulas.mem_imp hφ;
+
+end FormulaSet.SubformulaClosed
+
+end LO.Modal
